Reorganise botworld_quoteLib slightly; make it build

botworld_quoteLib.sml
@@ -1,16 +1,32 @@
+structure botworld_quoteLib = struct
+
 open preamble botworldTheory botworld_dataTheory
 open basicReflectionLib holSyntaxSyntax listSyntax
 
+val _ = Parse.temp_bring_to_front_overload","{Name=",",Thy="pair"}
 
-val _ = bring_to_front_overload","{Name=",",Thy="pair"}
+(* TODO: move to preamble *)
+fun term_rewrite eqs tm =
+  let
+    fun match_and_subst tm eq =
+      let val (s1,s2) = match_term (lhs eq) tm in mk_thm([],subst s1 (inst s2 eq)) end
+    fun rw1 tm = tryfind (match_and_subst tm) eqs
+  in tm |> QCONV (DEPTH_CONV rw1) |> concl |> rhs end
+(* -- *)
 
-val _ = Parse.overload_on("Num", ``Tyapp(strlit"num")[]``)
-val _ = Parse.overload_on("Level", ``Tyapp(strlit"level")[]``)
-val _ = Parse.overload_on("Pair", ``λt1 t2. Tyapp(strlit"prod")[t1;t2]``)
-
+(* TODO: move? *)
 fun assoc [] k = NONE
   | assoc ((k',v)::ls) k = if k = k' then SOME v else assoc ls k
+(* -- *)
 
+val _ = Parse.temp_overload_on("Num", ``Tyapp(strlit"num")[]``)
+val _ = Parse.temp_overload_on("Level", ``Tyapp(strlit"level")[]``)
+val _ = Parse.temp_overload_on("Pair", ``λt1 t2. Tyapp(strlit"prod")[t1;t2]``)
+
+(*
+quote_foo : (('a -> term) # type) -> (('a foo -> term) # type)
+quote_bar : ((('a -> term) # type), (('b -> term) # type)) -> ((('a, 'b) bar -> term) # type)
+*)
 
 fun quoter table (current_quote_ty,current_ty) ty =
   let
@@ -62,15 +78,7 @@ fun quote_term_to_deep table current_quote (type_being_defined,quote_ty_aux) =
           end
   in ttd end
 
-
 val aux_rws = ref ([]:term list)
-
-fun term_rewrite eqs tm = 
-  let 
-    fun match_and_subst tm eq =
-      let val (s1,s2) = match_term (lhs eq) tm in mk_thm([],subst s1 (inst s2 eq)) end
-    fun rw1 tm = tryfind (match_and_subst tm) eqs
-  in tm |> QCONV (DEPTH_CONV rw1) |> concl |> rhs end
 
 val mk_quote_tac = ref(NO_TAC)
 
@@ -104,7 +112,7 @@ fun mk_quote vnames ty =
     val quote_ty_name = "quote_"^tyname
     val quote_ty_aux_name = quote_ty_name^"_aux"
     val (v,b0) = ax |> SPEC_ALL |> concl |> inst [target_ty|->holSyntaxSyntax.term_ty]
-                    |> boolSyntax.dest_exists 
+                    |> boolSyntax.dest_exists
     val b = b0 |> strip_exists |> #2 |> strip_conj |> filter (fn s => v = rator (lhs (#2 (strip_forall s))))
     val (argts,argqs) =
       case vnames of NONE =>
@@ -132,7 +140,8 @@ fun mk_quote vnames ty =
       quote_term_to_deep table (mk_pair(quote_ty_aux_applied, inner_ty)) (ty,quote_ty_aux_applied) (rand l)
     val eqs = map (fn l => mk_eq(l,mk_rhs l |> term_rewrite (!aux_rws))) lhses
     val aux_def = Define [ANTIQUOTE(list_mk_conj eqs)]
-                  handle HOL_ERR _ => tDefine (quote_ty_name^"_def") [ANTIQUOTE(list_mk_conj eqs)] (!mk_quote_tac) before ignore (drop())
+                  handle HOL_ERR _ => tDefine (quote_ty_name^"_def") [ANTIQUOTE(list_mk_conj eqs)] (!mk_quote_tac)
+                                      before ignore (proofManagerLib.drop())
     val quote_ty = mk_var(quote_ty_name,
                               if null tyvs then
                                 mk_prod(type_of quote_ty_aux,type_ty)
@@ -151,87 +160,4 @@ fun mk_quote vnames ty =
    (aux_def,q_def)
   end
 
-val (quote_num_aux_def,quote_num_def) = mk_quote NONE ``:num``
-val (quote_level_aux_def,quote_level_def) = mk_quote NONE ``:level``
-val (quote_prod_aux_def,quote_prod_def) = mk_quote (SOME(["q1","q2"],["t1","t2"])) ``:'a # 'b``
-val (quote_list_aux_def,quote_list_def) = mk_quote (SOME(["q"],["t"])) ``:'a list``
-
-val quote_list_aux_cong = Q.store_thm("quote_list_aux_cong",`!l1 l2 t1 t2 q1 q2.
-l1 = l2 /\
-t1 = t2 /\
-(!a. MEM a l1 ==> q1 a = q2 a)
-==> quote_list_aux (q1,t1) l1 = quote_list_aux (q2,t2) l2`,
-Induct \\ rw[quote_list_aux_def] \\ rw[quote_list_aux_def]
-)
-
-val quote_list_is_aux = Q.prove(`FST (quote_list (x,y)) z = quote_list_aux (x,y) z`, rw[quote_list_def])
-
-val _ = DefnBase.export_cong "quote_list_aux_cong"
-val _ = aux_rws := concl quote_list_is_aux :: !aux_rws
-
-val quote_char_aux_def = Define `quote_char_aux c = Comb ^(term_to_deep ``CHR``) (quote_num_aux (ORD c))`
-val quote_char_def = Define `quote_char = (quote_char_aux , ^(type_to_deep ``:char``))`
-
-val (quote_id_aux_def,quote_id_def) = mk_quote (SOME(["q"],["t"])) ``:'a id``
-val (quote_tctor_aux_def,quote_tctor_def) = mk_quote NONE ``:tctor``
-
-val _ = mk_quote_tac := (wf_rel_tac `measure t_size` \\ gen_tac \\ Induct \\ rw[astTheory.t_size_def]
-                                   \\ simp[] \\ res_tac \\ simp[])
-
-val (quote_t_aux_def,quote_t_def) = mk_quote NONE ``:t`` 
-val quote_t_aux_def = save_thm("quote_t_aux_def",quote_t_aux_def |> REWRITE_RULE[GSYM quote_list_is_aux,ETA_AX])
-
-val (quote_spec_aux_def,quote_spec_def) = mk_quote NONE ``:spec``
-val (quote_option_aux_def,quote_option_def) = mk_quote (SOME(["q"],["t"])) ``:'a option``
-val _ = overload_on("quote_specs",``quote_list quote_spec``)
-
-val quote_int_aux_def = Define `quote_int_aux i = if i < 0i
-                                                  then Comb ^(term_to_deep ``int_neg``)
-                                                      (Comb ^(term_to_deep ``int_of_num``) (FST quote_num (Num (-i))))
-                                                  else Comb ^(term_to_deep ``int_of_num``) (FST quote_num (Num i))`
-val quote_int_def = Define `quote_int = (quote_int_aux, ^(type_to_deep ``:int``))`
-
-val quote_lit = Define `quote_lit = (ARB:lit->term,ARB:type) (* TODO *)`
-
-(* val quote_word_aux_def = Define `quote_word_aux ((q:'a -> term),t) (w:'a word) = Comb (Const (strlit "n2w") *)
-(*     (Fun Num (Tyapp (strlit "cart") [Bool; t]))) (FST quote_num (w2n w))` *)
-(* val quote_word_def = Define `quote_word (q,t) = (quote_word_aux (q,t) , type)` *)
-(* val _ = overload_on("quote_word8",``) *)
-
-val _ = mk_quote_tac := (wf_rel_tac `measure pat_size` \\ gen_tac \\ Induct \\ rw[astTheory.pat_size_def]
-                                   \\ simp[] \\ res_tac \\ simp[])
-val (quote_pat_aux_def,quote_pat_def) = mk_quote NONE ``:pat``
-val quote_pat_aux_def = save_thm("quote_t_aux_def",quote_pat_aux_def |> REWRITE_RULE[GSYM quote_list_is_aux,ETA_AX])
-
-val (quote_opn_aux_def,quote_opn_def) = mk_quote NONE ``:opn``
-val (quote_opb_aux_def,quote_opb_def) = mk_quote NONE ``:opb``
-val (quote_op_aux_def,quote_op_def) = mk_quote NONE ``:op``
-val (quote_lop_aux_def,quote_lop_def) = mk_quote NONE ``:lop``
-
-val _ = mk_quote_tac := (wf_rel_tac `measure exp_size` \\ rpt conj_tac \\ simp[] \\ (* TODO *)
-
-val (quote_exp_aux_def,quote_exp_def) = mk_quote NONE ``:exp``
-val (quote_dec_aux_def,quote_dec_def) = mk_quote NONE ``:dec``
-val _ = overload_on("quote_decs",``quote_list quote_dec``)
-
-val (quote_top_aux_def,quote_top_def) = mk_quote NONE ``:top``
-
-val (quote_command_aux_def,quote_command_def) = mk_quote NONE ``:command``
-
-val quote_top_def = Define`
-  quote_top = (ARB:top->term,ARB:type) (* TODO *)`;
-
-Val _ = overload_on("quote_prog",``quote_list quote_top``);
-
-val (quote_privateData_aux_def,quote_privateData_def) = mk_quote NONE ``:privateData``
-
-val quote_event_def = Define`
-  quote_event = (ARB:event->term,ARB:type) (* TODO *)`;
-
-val _ = overload_on("quote_observation",
-    ``quote_prod (quote_num,(quote_prod (quote_event,quote_privateData)))``);
-
-(*
-quote_foo : (('a -> term) # type) -> (('a foo -> term) # type)
-quote_bar : ((('a -> term) # type), (('b -> term) # type)) -> ((('a, 'b) bar -> term) # type)
-*)
+end
