botworld_quoteScript.sml
@@ -1,0 +1,89 @@
+open preamble botworld_quoteLib
+
+val _ = new_theory"botworld_quote";
+
+val (quote_num_aux_def,quote_num_def) = mk_quote NONE ``:num``
+val (quote_level_aux_def,quote_level_def) = mk_quote NONE ``:level``
+val (quote_prod_aux_def,quote_prod_def) = mk_quote (SOME(["q1","q2"],["t1","t2"])) ``:'a # 'b``
+val (quote_list_aux_def,quote_list_def) = mk_quote (SOME(["q"],["t"])) ``:'a list``
+
+val quote_list_aux_cong = Q.store_thm("quote_list_aux_cong",`!l1 l2 t1 t2 q1 q2.
+l1 = l2 /\
+t1 = t2 /\
+(!a. MEM a l1 ==> q1 a = q2 a)
+==> quote_list_aux (q1,t1) l1 = quote_list_aux (q2,t2) l2`,
+Induct \\ rw[quote_list_aux_def] \\ rw[quote_list_aux_def]
+)
+
+val quote_list_is_aux = Q.prove(`FST (quote_list (x,y)) z = quote_list_aux (x,y) z`, rw[quote_list_def])
+
+val _ = DefnBase.export_cong "quote_list_aux_cong"
+val _ = aux_rws := concl quote_list_is_aux :: !aux_rws
+
+val quote_char_aux_def = Define `quote_char_aux c = Comb ^(term_to_deep ``CHR``) (quote_num_aux (ORD c))`
+val quote_char_def = Define `quote_char = (quote_char_aux , ^(type_to_deep ``:char``))`
+
+val (quote_id_aux_def,quote_id_def) = mk_quote (SOME(["q"],["t"])) ``:'a id``
+val (quote_tctor_aux_def,quote_tctor_def) = mk_quote NONE ``:tctor``
+
+val _ = mk_quote_tac := (wf_rel_tac `measure t_size` \\ gen_tac \\ Induct \\ rw[astTheory.t_size_def]
+                                   \\ simp[] \\ res_tac \\ simp[])
+
+val (quote_t_aux_def,quote_t_def) = mk_quote NONE ``:t``
+val quote_t_aux_def = save_thm("quote_t_aux_def",quote_t_aux_def |> REWRITE_RULE[GSYM quote_list_is_aux,ETA_AX])
+
+val (quote_spec_aux_def,quote_spec_def) = mk_quote NONE ``:spec``
+val (quote_option_aux_def,quote_option_def) = mk_quote (SOME(["q"],["t"])) ``:'a option``
+val _ = overload_on("quote_specs",``quote_list quote_spec``)
+
+val quote_int_aux_def = Define `quote_int_aux i = if i < 0i
+                                                  then Comb ^(term_to_deep ``int_neg``)
+                                                      (Comb ^(term_to_deep ``int_of_num``) (FST quote_num (Num (-i))))
+                                                  else Comb ^(term_to_deep ``int_of_num``) (FST quote_num (Num i))`
+val quote_int_def = Define `quote_int = (quote_int_aux, ^(type_to_deep ``:int``))`
+
+val quote_lit = Define `quote_lit = (ARB:lit->term,ARB:type) (* TODO *)`
+
+(* val quote_word_aux_def = Define `quote_word_aux ((q:'a -> term),t) (w:'a word) = Comb (Const (strlit "n2w") *)
+(*     (Fun Num (Tyapp (strlit "cart") [Bool; t]))) (FST quote_num (w2n w))` *)
+(* val quote_word_def = Define `quote_word (q,t) = (quote_word_aux (q,t) , type)` *)
+(* val _ = overload_on("quote_word8",``) *)
+
+val _ = mk_quote_tac := (wf_rel_tac `measure pat_size` \\ gen_tac \\ Induct \\ rw[astTheory.pat_size_def]
+                                   \\ simp[] \\ res_tac \\ simp[])
+val (quote_pat_aux_def,quote_pat_def) = mk_quote NONE ``:pat``
+val quote_pat_aux_def = save_thm("quote_t_aux_def",quote_pat_aux_def |> REWRITE_RULE[GSYM quote_list_is_aux,ETA_AX])
+
+val (quote_opn_aux_def,quote_opn_def) = mk_quote NONE ``:opn``
+val (quote_opb_aux_def,quote_opb_def) = mk_quote NONE ``:opb``
+val (quote_op_aux_def,quote_op_def) = mk_quote NONE ``:op``
+val (quote_lop_aux_def,quote_lop_def) = mk_quote NONE ``:lop``
+
+(*
+val _ = mk_quote_tac := (wf_rel_tac `measure exp_size` \\ rpt conj_tac \\ simp[])
+
+val (quote_exp_aux_def,quote_exp_def) = mk_quote NONE ``:exp``
+*)
+val quote_exp = Define `quote_exp = (ARB:exp->term,ARB:type) (* TODO *)`
+
+val (quote_dec_aux_def,quote_dec_def) = mk_quote NONE ``:dec``
+val _ = overload_on("quote_decs",``quote_list quote_dec``)
+
+val (quote_top_aux_def,quote_top_def) = mk_quote NONE ``:top``
+
+val (quote_command_aux_def,quote_command_def) = mk_quote NONE ``:command``
+
+val quote_top_def = Define`
+  quote_top = (ARB:top->term,ARB:type) (* TODO *)`;
+
+val _ = overload_on("quote_prog",``quote_list quote_top``);
+
+val (quote_privateData_aux_def,quote_privateData_def) = mk_quote NONE ``:privateData``
+
+val quote_event_def = Define`
+  quote_event = (ARB:event->term,ARB:type) (* TODO *)`;
+
+val _ = overload_on("quote_observation",
+    ``quote_prod (quote_num,(quote_prod (quote_event,quote_privateData)))``);
+
+val _ = export_theory();
